checkpoint cleanup

src/Spec/Equiv.v
@@ -3,6 +3,10 @@ Require Import Relations.Relation_Operators.
 Require Import RelationClasses.
 Require Import Morphisms.
 Require Import Helpers.Helpers.
+Require Import Helpers.ListStuff.
+Require Import List.
+
+Import ListNotations.
 
 Global Set Implicit Arguments.
 Global Generalizable All Variables.
@@ -46,8 +50,8 @@ Fixpoint trace_filter_hi `(t : trace opLoT opHiT) : trace opLoT opHiT :=
 Definition trace_match_hi {opLoT opHiT} (t1 t2 : trace opLoT opHiT) :=
   trace_filter_hi t1 = trace_filter_hi t2.
 
-Instance trace_match_hi_preorder {opLoT opHiT} :
-  PreOrder `(@trace_match_hi opLoT opHiT).
+Instance trace_match_hi_preorder :
+  PreOrder (@trace_match_hi opLoT opHiT).
 Proof.
   split.
   - firstorder.
@@ -82,37 +86,15 @@ Proof.
   unfold trace_match_hi; simpl; eauto.
 Qed.
 
+Lemma trace_match_hi_refl : forall `(tr : trace opT opHiT),
+  trace_match_hi tr tr.
+Proof.
+  reflexivity.
+Qed.
+
 Hint Resolve trace_match_hi_drop_lo_l.
 Hint Resolve trace_match_hi_drop_lo_r.
-
-
-(** Preserving traces for an entire threads_state *)
-
-Definition same_traces_s {opLo opHi State} op_step (s s' : State) (ts1 ts2 : @threads_state opLo opHi) :=
-  forall tr,
-    exec op_step s ts1 tr ->
-    exists tr', exec op_step s' ts2 tr' /\
-      trace_match_hi tr tr'.
-
-Definition same_traces {opLo opHi State} op_step (s : State) (ts1 ts2 : @threads_state opLo opHi) :=
-  same_traces_s op_step s s ts1 ts2.
-
-
-Instance same_traces_preorder {opT opHiT State op_step s} :
-  PreOrder (@same_traces opT opHiT State op_step s).
-Proof.
-  split.
-  - unfold Reflexive.
-    unfold same_traces, same_traces_s; intros.
-    eexists; intuition eauto.
-    reflexivity.
-  - unfold Transitive.
-    unfold same_traces, same_traces_s; intros.
-    eapply H in H1. deex.
-    eapply H0 in H1. deex.
-    eexists; intuition eauto.
-    etransitivity; eauto.
-Qed.
+Hint Resolve trace_match_hi_refl.
 
 
 (** A strong notion of execution equivalence, independent of semantics *)
@@ -129,61 +111,827 @@ Definition exec_equiv_opt `(p1 : maybe_proc opT opHiT) p2 :=
 Definition exec_equiv `(p1 : proc opT opHiT T) (p2 : proc _ _ T) :=
   exec_equiv_opt (Proc p1) (Proc p2).
 
-Instance exec_equiv_ts_preorder {opLoT opHiT} :
-  PreOrder (@exec_equiv_ts opLoT opHiT).
+Instance exec_equiv_ts_equivalence :
+  Equivalence (@exec_equiv_ts opLoT opHiT).
 Proof.
   split.
   - firstorder.
+  - unfold Symmetric, exec_equiv_ts; intros.
+    split; intros; apply H; eauto.
   - unfold Transitive, exec_equiv_ts; intros.
     split; intros.
     + apply H0. apply H. eauto.
     + apply H. apply H0. eauto.
 Qed.
 
+Theorem exec_equiv_ts_app_None : forall `(ts : @threads_state opT opHiT),
+  exec_equiv_ts ts (ts ++ [NoProc]).
+Proof.
+  split; intros.
+  - induction H.
+    + eapply ExecOne with (tid := tid); eauto.
+      eapply thread_get_app_NoProc in H; eauto.
+      erewrite <- thread_upd_app_NoProc; eauto.
+    + eapply ExecEmpty.
+      eapply no_runnable_threads_app_NoProc in H; eauto.
+  - remember (ts ++ [NoProc]); generalize dependent ts;
+      induction H; intros; subst.
+    + eapply ExecOne with (tid := tid); eauto.
+      eapply thread_get_app_NoProc; eauto.
+      eapply IHexec.
+      erewrite thread_upd_app_NoProc; eauto.
+      eapply thread_get_app_NoProc in H. eauto.
+    + eapply ExecEmpty.
+      eapply no_runnable_threads_app_NoProc; eauto.
+Qed.
 
-(** Preserving traces for a single thread *)
+Theorem exec_equiv_ts_pad : forall n `(ts : @threads_state opT opHiT),
+  exec_equiv_ts ts (pad ts n NoProc).
+Proof.
+  intros.
+  rewrite pad_is_append.
+  generalize (n - length ts); intros.
+  rewrite <- rev_repeat.
+  induction n0; simpl.
+  - rewrite app_nil_r. reflexivity.
+  - rewrite app_assoc.
+    etransitivity.
+    2: eapply exec_equiv_ts_app_None.
+    eauto.
+Qed.
 
-Definition trace_equiv_s `(s : State) s' tid `(op_step : OpSemantics opT State) `(p1 : proc opT opHiT T) (p2 : proc _ _ T) :=
-  forall ts,
-    same_traces_s op_step s s'
-      (ts [[ tid := Proc p1 ]])
-      (ts [[ tid := Proc p2 ]]).
-
-Definition trace_equiv {opT opHiT T} `(op_step : OpSemantics opT State) (p1 p2 : proc opT opHiT T) :=
-  forall ts s tid,
-    same_traces op_step s
-      (ts [[ tid := Proc p1 ]])
-      (ts [[ tid := Proc p2 ]]).
-
-
-Instance trace_equiv_preorder {opT opHiT T State op_step} :
-  PreOrder (@trace_equiv opT opHiT T State op_step).
+Instance exec_equiv_opt_equivalence :
+  Equivalence (@exec_equiv_opt opLoT opHiT).
 Proof.
   split.
-  - unfold Reflexive; intros.
-    unfold trace_equiv; intros.
+  - unfold exec_equiv_opt, Reflexive; intros.
     reflexivity.
+  - unfold exec_equiv_opt, Symmetric; intros.
+    symmetry. eauto.
+  - intros t1 t2 t3.
+    unfold exec_equiv; split; intros.
+    + eapply H in H1; eauto.
+      eapply H0 in H1.
+      eauto.
+    + eapply H; eauto.
+      eapply H0; eauto.
+Qed.
+
+Instance exec_equiv_equivalence :
+  Equivalence (@exec_equiv opLoT opHiT T).
+Proof.
+  unfold exec_equiv.
+  split.
+  - intro t.
+    reflexivity.
+  - unfold Symmetric, exec_equiv_opt; intros.
+    symmetry. eauto.
   - unfold Transitive; intros.
-    unfold trace_equiv; intros.
     etransitivity; eauto.
 Qed.
 
-Instance trace_equiv_proper {opT opHiT T State op_step} :
-  Proper (Basics.flip (@trace_equiv opT opHiT T State op_step) ==>
-          @trace_equiv opT opHiT T State op_step ==>
-          Basics.impl) (@trace_equiv opT opHiT T State op_step).
+Instance thread_upd_exec_equiv_proper :
+  Proper (eq ==> eq ==> exec_equiv_opt ==> exec_equiv_ts) (@thread_upd opT opHiT).
 Proof.
+  intros.
+  intros ts0 ts1 H; subst.
+  intros tid tid' H'; subst.
+  intros o0 o1 H'.
+
+  unfold exec_equiv_ts; split; intros.
+  - apply H'; eauto.
+  - apply H'; eauto.
+Qed.
+
+Instance Proc_exec_equiv_proper :
+  Proper (exec_equiv ==> exec_equiv_opt) (@Proc opT opHiT T).
+Proof.
+  intros.
+  unfold exec_equiv.
+  intros ts0 ts1 H; subst.
+  eauto.
+Qed.
+
+Theorem exec_equiv_ret_bind : forall `(v : T) `(p : T -> proc opT opHiT T'),
+  exec_equiv (Bind (Ret v) p) (p v).
+Proof.
+  split; intros.
+  - match goal with
+    | H : exec _ _ (thread_upd ?ts ?tid (Proc ?p)) _ |- _ =>
+      remember (thread_upd ts tid (Proc p));
+      generalize dependent ts;
+      induction H; intros; subst
+    end.
+    + destruct (tid0 == tid); subst; autorewrite with t in *.
+      * repeat maybe_proc_inv; repeat exec_tid_inv.
+        simpl. eauto.
+
+      * eapply ExecOne with (tid := tid0).
+          rewrite thread_upd_ne in * by auto. eauto.
+          eauto.
+        rewrite thread_upd_upd_ne by eauto.
+        eapply IHexec.
+        rewrite thread_upd_upd_ne; eauto.
+    + exfalso; eapply thread_upd_not_empty; eauto.
+
+  - match goal with
+    | H : exec _ _ (thread_upd ?ts ?tid (Proc ?p)) _ |- _ =>
+      remember (thread_upd ts tid (Proc p));
+      generalize dependent ts;
+      induction H; intros; subst
+    end.
+    + destruct (tid0 == tid); subst.
+      * autorewrite with t in *.
+        repeat maybe_proc_inv.
+        rewrite <- app_nil_l with (l := evs).
+        rewrite prepend_app.
+        eapply ExecOne with (tid := tid).
+          autorewrite with t; eauto.
+          eauto.
+          autorewrite with t.
+        eapply ExecOne with (tid := tid).
+          autorewrite with t; eauto.
+          eauto.
+          autorewrite with t.
+        eauto.
+
+      * eapply ExecOne with (tid := tid0).
+          autorewrite with t in *; eauto.
+          eauto.
+          rewrite thread_upd_upd_ne by eauto.
+        eapply IHexec.
+        rewrite thread_upd_upd_ne by auto.
+        eauto.
+
+    + specialize (H tid).
+      rewrite thread_upd_eq in H.
+      congruence.
+Qed.
+
+Theorem exec_equiv_ret_None : forall opT opHiT `(v : T),
+  @exec_equiv_opt opT opHiT (Proc (Ret v)) NoProc.
+Proof.
+  split; intros.
+  - match goal with
+    | H : exec _ _ (thread_upd ?ts ?tid (Proc ?p)) _ |- _ =>
+      remember (thread_upd ts tid (Proc p));
+      generalize dependent ts;
+      induction H; intros; subst
+    end.
+    + destruct (tid0 == tid); subst.
+      * autorewrite with t in *.
+        repeat maybe_proc_inv.
+        repeat exec_tid_inv.
+        simpl. eauto.
+
+      * rewrite thread_upd_upd_ne in * by eauto.
+        eapply ExecOne with (tid := tid0).
+          rewrite thread_upd_ne in * by auto. eauto.
+          eauto.
+        rewrite thread_upd_upd_ne by auto.
+        eauto.
+    + specialize (H tid).
+      rewrite thread_upd_eq in H.
+      congruence.
+
+  - replace tr with (prepend tid nil tr) by reflexivity.
+    eapply ExecOne with (tid := tid).
+      rewrite thread_upd_eq. eauto.
+      eauto.
+    autorewrite with t.
+    eauto.
+Qed.
+
+Theorem exec_equiv_bind_ret : forall `(p : proc opT opHiT T),
+  exec_equiv (Bind p Ret) p.
+Proof.
+  unfold exec_equiv; split; intros.
+  - match goal with
+    | H : exec _ _ (thread_upd ?ts ?tid (Proc ?pp)) _ |- _ =>
+      remember (thread_upd ts tid (Proc pp));
+      generalize dependent ts;
+      generalize dependent p;
+      induction H; intros; subst
+    end.
+    + destruct (tid0 == tid); subst.
+      * autorewrite with t in *.
+        repeat maybe_proc_inv.
+        exec_tid_inv.
+        eapply ExecOne with (tid := tid).
+          rewrite thread_upd_eq in * by auto. eauto.
+          eauto.
+        autorewrite with t.
+
+        destruct result0; eauto.
+
+        eapply exec_equiv_ret_None in H1.
+        eauto.
+
+      * rewrite thread_upd_upd_ne in * by eauto.
+        eapply ExecOne with (tid := tid0).
+          rewrite thread_upd_ne in * by auto. eauto.
+          eauto.
+        rewrite thread_upd_upd_ne by auto.
+        eauto.
+    + specialize (H tid).
+      rewrite thread_upd_eq in H.
+      congruence.
+
+  - match goal with
+    | H : exec _ _ (thread_upd ?ts ?tid (Proc ?pp)) _ |- _ =>
+      remember (thread_upd ts tid (Proc pp));
+      generalize dependent ts;
+      generalize dependent p;
+      induction H; intros; subst
+    end.
+    + destruct (tid0 == tid); subst.
+      * autorewrite with t in *.
+        repeat maybe_proc_inv.
+        eapply ExecOne with (tid := tid).
+          rewrite thread_upd_eq. eauto.
+          eauto.
+        autorewrite with t in *.
+        destruct result; eauto.
+        apply exec_equiv_ret_None; eauto.
+
+      * rewrite thread_upd_upd_ne in * by eauto.
+        eapply ExecOne with (tid := tid0).
+          rewrite thread_upd_ne in * by auto. eauto.
+          eauto.
+        rewrite thread_upd_upd_ne by auto.
+        eauto.
+    + specialize (H tid).
+      rewrite thread_upd_eq in H.
+      congruence.
+Qed.
+
+Theorem exec_equiv_bind_bind : forall `(p1 : proc opT opHiT T1) `(p2 : T1 -> proc opT opHiT T2) `(p3 : T2 -> proc opT opHiT T3),
+  exec_equiv (Bind (Bind p1 p2) p3) (Bind p1 (fun v => Bind (p2 v) p3)).
+Proof.
+  unfold exec_equiv; split; intros.
+  - match goal with
+    | H : exec _ _ (thread_upd ?ts ?tid (Proc ?p)) _ |- _ =>
+      remember (thread_upd ts tid (Proc p));
+      generalize dependent ts;
+      generalize dependent p1;
+      induction H; intros; subst
+    end.
+    + destruct (tid0 == tid); subst.
+      * autorewrite with t in *.
+        repeat maybe_proc_inv.
+        exec_tid_inv.
+        exec_tid_inv.
+        eapply ExecOne with (tid := tid).
+          rewrite thread_upd_eq. eauto.
+          eauto.
+        autorewrite with t.
+
+        destruct result; eauto.
+
+      * eapply ExecOne with (tid := tid0).
+          autorewrite with t in *; eauto.
+          eauto.
+        rewrite thread_upd_upd_ne by auto.
+        eapply IHexec.
+        rewrite thread_upd_upd_ne; eauto.
+    + specialize (H tid).
+      rewrite thread_upd_eq in H.
+      congruence.
+
+  - match goal with
+    | H : exec _ _ (thread_upd ?ts ?tid (Proc ?p)) _ |- _ =>
+      remember (thread_upd ts tid (Proc p));
+      generalize dependent ts;
+      generalize dependent p1;
+      induction H; intros; subst
+    end.
+    + destruct (tid0 == tid); subst.
+      * autorewrite with t in *.
+        repeat maybe_proc_inv.
+        exec_tid_inv.
+
+        eapply ExecOne with (tid := tid).
+          rewrite thread_upd_eq. eauto.
+          eauto.
+        autorewrite with t.
+
+        destruct result0; eauto.
+
+      * rewrite thread_upd_upd_ne in * by eauto.
+        eapply ExecOne with (tid := tid0).
+          rewrite thread_upd_ne in * by auto. eauto.
+          eauto.
+        rewrite thread_upd_upd_ne by auto.
+        eauto.
+    + specialize (H tid).
+      rewrite thread_upd_eq in H.
+      congruence.
+Qed.
+
+Theorem exec_equiv_bind_a : forall `(p : proc opT opHiT T) `(p1 : T -> proc _ _ T') p2,
+  (forall x, exec_equiv (p1 x) (p2 x)) ->
+  exec_equiv (Bind p p1) (Bind p p2).
+Proof.
+  unfold exec_equiv; split; intros.
+  - match goal with
+    | H : exec _ _ (thread_upd ?ts ?tid (Proc ?pp)) _ |- _ =>
+      remember (thread_upd ts tid (Proc pp));
+      generalize dependent ts;
+      generalize dependent p;
+      induction H; intros; subst
+    end.
+    + destruct (tid0 == tid); subst.
+      * autorewrite with t in *.
+        repeat maybe_proc_inv.
+        exec_tid_inv.
+        eapply ExecOne with (tid := tid).
+          rewrite thread_upd_eq. eauto.
+          eauto.
+        autorewrite with t.
+
+        destruct result0; eauto.
+        eapply H in H2; eauto.
+
+      * eapply ExecOne with (tid := tid0).
+          autorewrite with t in *; eauto.
+          eauto.
+        rewrite thread_upd_upd_ne by auto.
+        eapply IHexec.
+        rewrite thread_upd_upd_ne; eauto.
+    + exfalso; eauto.
+
+  - match goal with
+    | H : exec _ _ (thread_upd ?ts ?tid (Proc ?pp)) _ |- _ =>
+      remember (thread_upd ts tid (Proc pp));
+      generalize dependent ts;
+      generalize dependent p;
+      induction H; intros; subst
+    end.
+    + destruct (tid0 == tid); subst.
+      * autorewrite with t in *.
+        repeat maybe_proc_inv.
+        exec_tid_inv.
+        eapply ExecOne with (tid := tid).
+          rewrite thread_upd_eq. eauto.
+          eauto.
+        autorewrite with t.
+
+        destruct result0; eauto.
+        eapply H in H2; eauto.
+
+      * eapply ExecOne with (tid := tid0).
+          autorewrite with t in *; eauto.
+          eauto.
+        rewrite thread_upd_upd_ne by auto.
+        eapply IHexec.
+        rewrite thread_upd_upd_ne; eauto.
+    + exfalso; eauto.
+Qed.
+
+Theorem exec_equiv_bind_bind' : forall `(p1 : proc opT opHiT T1) `(p2 : T1 -> proc _ _ T2) `(p3 : T1 -> T2 -> proc _ _ T3),
+  exec_equiv (Bind p1 (fun x => Bind (p2 x) (p3 x)))
+             (Bind (Bind p1 (fun x => Bind (p2 x) (fun y => Ret (x, y))))
+                   (fun p => p3 (fst p) (snd p))).
+Proof.
+  intros.
+  rewrite exec_equiv_bind_bind.
+  eapply exec_equiv_bind_a; intros.
+  rewrite exec_equiv_bind_bind.
+  eapply exec_equiv_bind_a; intros.
+  rewrite exec_equiv_ret_bind; simpl.
+  reflexivity.
+Qed.
+
+Instance Bind_exec_equiv_proper_2 :
+  Proper (eq ==>
+          pointwise_relation T0 exec_equiv ==>
+          @exec_equiv opT opHiT T) Bind.
+Proof.
+  intros.
+  intros p1a p1b H1; subst.
+  intros p2a p2b H2.
+  eapply exec_equiv_bind_a; intros.
+  eapply H2.
+Qed.
+
+
+(** Trace inclusion for an entire threads_state *)
+
+Definition hitrace_incl_ts_s {opLo opHi State} op_step (s s' : State) (ts1 ts2 : @threads_state opLo opHi) :=
+  forall tr,
+    exec op_step s ts1 tr ->
+    exists tr', exec op_step s' ts2 tr' /\
+      trace_match_hi tr tr'.
+
+Definition hitrace_incl_ts {opLo opHi State} op_step (s : State) (ts1 ts2 : @threads_state opLo opHi) :=
+  hitrace_incl_ts_s op_step s s ts1 ts2.
+
+Instance hitrace_incl_ts_preorder {opT opHiT State op_step s} :
+  PreOrder (@hitrace_incl_ts opT opHiT State op_step s).
+Proof.
+  split.
+  - unfold Reflexive.
+    unfold hitrace_incl_ts, hitrace_incl_ts_s; intros.
+    eexists; intuition eauto.
+  - unfold Transitive.
+    unfold hitrace_incl_ts, hitrace_incl_ts_s; intros.
+    eapply H in H1. deex.
+    eapply H0 in H1. deex.
+    eexists; intuition eauto.
+    etransitivity; eauto.
+Qed.
+
+
+(** Trace inclusion for a single thread *)
+
+Definition hitrace_incl_s `(s : State) s' tid `(op_step : OpSemantics opT State) `(p1 : proc opT opHiT T) (p2 : proc _ _ T) :=
+  forall ts,
+    hitrace_incl_ts_s op_step s s'
+      (ts [[ tid := Proc p1 ]])
+      (ts [[ tid := Proc p2 ]]).
+
+Definition hitrace_incl_opt {opT opHiT} `(op_step : OpSemantics opT State) p1 p2 :=
+  forall (ts : @threads_state opT opHiT) s tid,
+    hitrace_incl_ts op_step s
+      (ts [[ tid := p1 ]])
+      (ts [[ tid := p2 ]]).
+
+Definition hitrace_incl {opT opHiT T} `(op_step : OpSemantics opT State) (p1 p2 : proc opT opHiT T) :=
+  hitrace_incl_opt op_step (Proc p1) (Proc p2).
+
+
+Instance hitrace_incl_opt_preorder :
+  PreOrder (@hitrace_incl_opt opT opHiT State op_step).
+Proof.
+  split.
+  - unfold Reflexive; intros.
+    unfold hitrace_incl_opt; intros.
+    reflexivity.
+  - unfold Transitive; intros.
+    unfold hitrace_incl_opt; intros.
+    etransitivity; eauto.
+Qed.
+
+Instance hitrace_incl_preorder :
+  PreOrder (@hitrace_incl opT opHiT T State op_step).
+Proof.
+  split.
+  - unfold Reflexive; intros.
+    unfold hitrace_incl; intros.
+    reflexivity.
+  - unfold Transitive; intros.
+    unfold hitrace_incl; intros.
+    etransitivity; eauto.
+Qed.
+
+Instance hitrace_incl_proper :
+  Proper (Basics.flip (@hitrace_incl opT opHiT T State op_step) ==>
+          @hitrace_incl opT opHiT T State op_step ==>
+          Basics.impl) (@hitrace_incl opT opHiT T State op_step).
+Proof.
+  intros.
   intros p1 p2 H21 p3 p4 H34 H; subst.
   unfold Basics.flip in *.
   repeat (etransitivity; eauto).
 Qed.
 
-Instance trace_equiv_proper_flip {opT opHiT T State op_step} :
-  Proper (@trace_equiv opT opHiT T State op_step ==>
-          Basics.flip (@trace_equiv opT opHiT T State op_step) ==>
-          Basics.flip Basics.impl) (@trace_equiv opT opHiT T State op_step).
+Instance hitrace_incl_proper_flip :
+  Proper (@hitrace_incl opT opHiT T State op_step ==>
+          Basics.flip (@hitrace_incl opT opHiT T State op_step) ==>
+          Basics.flip Basics.impl) (@hitrace_incl opT opHiT T State op_step).
 Proof.
+  intros.
   intros p1 p2 H21 p3 p4 H34 H; subst.
   unfold Basics.flip in *.
   repeat (etransitivity; eauto).
+Qed.
+
+Instance hitrace_incl_s_proper :
+  Proper (Basics.flip (@hitrace_incl opT opHiT T State op_step) ==>
+          @hitrace_incl opT opHiT T State op_step ==>
+          Basics.impl) (@hitrace_incl_s State s s' tid opT op_step opHiT T).
+Proof.
+  intros.
+  intros p1 p2 H12 p3 p4 H34 H; subst.
+  unfold hitrace_incl_s, hitrace_incl_ts_s; intros.
+  apply H12 in H0. deex.
+  apply H in H0. deex.
+  apply H34 in H0. deex.
+  eexists; split.
+  eauto.
+  repeat ( etransitivity; eauto ).
+Qed.
+
+Instance hitrace_incl_s_proper_flip :
+  Proper (@hitrace_incl opT opHiT T State op_step ==>
+          Basics.flip (@hitrace_incl opT opHiT T State op_step) ==>
+          Basics.flip Basics.impl) (@hitrace_incl_s State s s' tid opT op_step opHiT T).
+Proof.
+  intros.
+  intros p1 p2 H12 p3 p4 H34 H; subst.
+  unfold hitrace_incl_s, hitrace_incl_ts_s; intros.
+  apply H12 in H0. deex.
+  apply H in H0. deex.
+  apply H34 in H0. deex.
+  eexists; split.
+  eauto.
+  repeat ( etransitivity; eauto ).
+Qed.
+
+Instance hitrace_incl_exec_equiv_proper :
+  Proper (exec_equiv ==> exec_equiv ==> iff)
+         (@hitrace_incl opT opHiT T State op_step).
+Proof.
+  intros p1 p1' ?.
+  intros p2 p2' ?.
+  split; intros.
+  - unfold hitrace_incl, hitrace_incl_opt,
+           hitrace_incl_ts, hitrace_incl_ts_s; intros.
+    apply H in H2.
+    apply H1 in H2.
+    deex.
+    apply H0 in H2.
+    eauto.
+  - unfold hitrace_incl, hitrace_incl_opt,
+           hitrace_incl_ts, hitrace_incl_ts_s; intros.
+    apply H in H2.
+    apply H1 in H2.
+    deex.
+    apply H0 in H2.
+    eauto.
+Qed.
+
+Instance hitrace_incl_s_exec_equiv_proper :
+  Proper (exec_equiv ==> exec_equiv ==> iff)
+         (@hitrace_incl_s State s s' tid opT op_step opHiT T).
+Proof.
+  intros.
+  intros p1 p1' ?.
+  intros p2 p2' ?.
+  split; intros.
+  - unfold hitrace_incl_s, hitrace_incl_ts_s; intros.
+    apply H in H2.
+    apply H1 in H2.
+    deex.
+    apply H0 in H2.
+    eauto.
+  - unfold hitrace_incl_s, hitrace_incl_ts_s; intros.
+    apply H in H2.
+    apply H1 in H2.
+    deex.
+    apply H0 in H2.
+    eauto.
+Qed.
+
+Instance Proc_hitrace_incl_proper :
+  Proper (@hitrace_incl opT opHiT T State op_step ==>
+          @hitrace_incl_opt opT opHiT State op_step) (@Proc opT opHiT T).
+Proof.
+  intros.
+  unfold exec_equiv.
+  intros ts0 ts1 H; subst.
+  eauto.
+Qed.
+
+Instance thread_upd_hitrace_incl_proper :
+  Proper (eq ==> eq ==>
+          @hitrace_incl_opt opT opHiT State op_step ==>
+          hitrace_incl_ts op_step s) (@thread_upd opT opHiT).
+Proof.
+  intros.
+  intros ts0 ts1 H; subst.
+  intros tid tid' H; subst.
+  intros p1 p2 H.
+
+  unfold hitrace_incl_opt in H.
+  eauto.
+Qed.
+
+Lemma hitrace_incl_opret :
+  forall `(p : T -> proc opT opHiT T') (v : T) `(op_step : OpSemantics opT State),
+  hitrace_incl op_step
+    (Bind (OpRet v) p)
+    (p v).
+Proof.
+  unfold hitrace_incl, hitrace_incl_opt,
+         hitrace_incl_ts, hitrace_incl_ts_s.
+  intros.
+
+  match goal with
+  | H : exec _ _ (thread_upd ?ts ?tid ?p) _ |- _ =>
+    remember (thread_upd ts tid p);
+    generalize dependent ts;
+    induction H; intros; subst
+  end.
+
+  - destruct (tid == tid0); subst.
+    + autorewrite with t in *.
+      repeat maybe_proc_inv.
+      exec_tid_inv.
+      exec_tid_inv.
+
+      eexists; split.
+      eauto.
+      constructor.
+
+    + edestruct IHexec; intuition idtac.
+      rewrite thread_upd_upd_ne; eauto.
+
+      autorewrite with t in *.
+      eexists; split.
+
+      eapply ExecOne with (tid := tid0).
+        autorewrite with t; eauto.
+        eauto.
+        rewrite thread_upd_upd_ne by assumption; eauto.
+      eauto.
+
+  - exfalso; eauto.
+Qed.
+
+Lemma hitrace_incl_opcall :
+  forall `(p : unit -> proc opT opHiT T') `(op : opT T) `(op_step : OpSemantics opT State),
+  hitrace_incl op_step
+    (Bind (OpCall op) p)
+    (p tt).
+Proof.
+  unfold hitrace_incl, hitrace_incl_opt,
+         hitrace_incl_ts, hitrace_incl_ts_s.
+  intros.
+
+  match goal with
+  | H : exec _ _ (thread_upd ?ts ?tid ?p) _ |- _ =>
+    remember (thread_upd ts tid p);
+    generalize dependent ts;
+    induction H; intros; subst
+  end.
+
+  - destruct (tid == tid0); subst.
+    + autorewrite with t in *.
+      repeat maybe_proc_inv.
+      exec_tid_inv.
+      exec_tid_inv.
+
+      eexists; intuition eauto.
+      constructor.
+
+    + edestruct IHexec; intuition idtac.
+      rewrite thread_upd_upd_ne; eauto.
+
+      autorewrite with t in *.
+      eexists; split.
+
+      eapply ExecOne with (tid := tid0).
+        autorewrite with t; eauto.
+        eauto.
+        rewrite thread_upd_upd_ne; eauto.
+      eauto.
+
+  - exfalso; eauto.
+Qed.
+
+Theorem hitrace_incl_opexec :
+  forall `(p : T -> proc opT opHiT T') op `(op_step : OpSemantics opT State),
+  hitrace_incl op_step
+    (Bind (OpExec op) p)
+    (Bind (Atomic (Op op)) p).
+Proof.
+  unfold hitrace_incl, hitrace_incl_opt,
+         hitrace_incl_ts, hitrace_incl_ts_s.
+  intros.
+
+  match goal with
+  | H : exec _ _ (thread_upd ?ts ?tid ?p) _ |- _ =>
+    remember (thread_upd ts tid p);
+    generalize dependent ts;
+    induction H; intros; subst
+  end.
+
+  - destruct (tid == tid0); subst.
+    + autorewrite with t in *.
+      repeat maybe_proc_inv.
+      repeat exec_tid_inv.
+
+      eexists; split.
+
+      eapply ExecOne with (tid := tid0).
+        autorewrite with t; eauto.
+        eauto 20.
+        autorewrite with t; eauto.
+
+      simpl; eauto.
+
+    + edestruct IHexec; intuition idtac.
+      rewrite thread_upd_upd_ne; eauto.
+
+      autorewrite with t in *.
+      eexists; split.
+
+      eapply ExecOne with (tid := tid0).
+        autorewrite with t; eauto.
+        eauto.
+        rewrite thread_upd_upd_ne; eauto.
+      eauto.
+
+  - exfalso; eauto.
+Qed.
+
+Theorem hitrace_incl_bind_a : forall `(p : proc opT opHiT T) `(p2 : T -> proc _ _ T') p2' `(op_step : OpSemantics opT State),
+  (forall x, hitrace_incl op_step (p2 x) (p2' x)) ->
+  hitrace_incl op_step (Bind p p2) (Bind p p2').
+Proof.
+  unfold hitrace_incl, hitrace_incl_opt,
+         hitrace_incl_ts, hitrace_incl_ts_s.
+  intros.
+
+  match goal with
+  | H : exec _ _ (thread_upd ?ts ?tid ?pp) _ |- _ =>
+    remember (thread_upd ts tid pp);
+    generalize dependent ts;
+    generalize dependent p;
+    induction H; intros; subst
+  end.
+
+  - destruct (tid0 == tid); subst.
+    + autorewrite with t in *.
+      repeat maybe_proc_inv.
+      exec_tid_inv.
+      destruct result0.
+
+      * edestruct H; eauto.
+        intuition idtac.
+
+        eexists; split.
+        eapply ExecOne with (tid := tid).
+          autorewrite with t; eauto.
+          eauto.
+          autorewrite with t; eauto.
+        eauto.
+
+      * edestruct IHexec; eauto.
+        intuition idtac.
+
+        eexists; split.
+        eapply ExecOne with (tid := tid).
+          autorewrite with t; eauto.
+          eauto.
+          autorewrite with t; eauto.
+        eauto.
+
+    + edestruct IHexec.
+      rewrite thread_upd_upd_ne; eauto.
+      intuition idtac.
+
+      autorewrite with t in *.
+      eexists; split.
+      eapply ExecOne with (tid := tid0).
+        autorewrite with t; eauto.
+        eauto.
+        rewrite thread_upd_upd_ne; eauto.
+      eauto.
+  - exfalso; eauto.
+Qed.
+
+Theorem hitrace_incl_bind : forall `(p1 : proc opT opHiT T1) p1' `(p2 : T1 -> proc _ _ T2) p2' `(op_step : OpSemantics opT State),
+  (forall `(rx : _ -> proc _ _ T),
+    hitrace_incl op_step (Bind p1 rx) (Bind p1' rx)) ->
+  (forall `(rx : _ -> proc _ _ T) x,
+    hitrace_incl op_step (Bind (p2 x) rx) (Bind (p2' x) rx)) ->
+  forall `(rx : _ -> proc _ _ T),
+    hitrace_incl op_step (Bind (Bind p1 p2) rx) (Bind (Bind p1' p2') rx).
+Proof.
+  intros.
+  repeat rewrite exec_equiv_bind_bind.
+  rewrite H.
+  eapply hitrace_incl_bind_a.
+  eauto.
+Qed.
+
+Instance Bind_hitrace_incl_proper_2 :
+  Proper (eq ==>
+          pointwise_relation T0 (@hitrace_incl opT opHiT T State op_step) ==>
+          @hitrace_incl opT opHiT T State op_step) Bind.
+Proof.
+  intros.
+  intros p1a p1b H1; subst.
+  intros p2a p2b H2.
+  eapply hitrace_incl_bind_a; intros.
+  eapply H2.
+Qed.
+
+Theorem hitrace_incl_op :
+  forall `(p : T -> proc opT opHiT T') op `(op_step : OpSemantics opT State),
+  hitrace_incl op_step
+    (Bind (Op op) p)
+    (Bind (Atomic (Op op)) p).
+Proof.
+  intros.
+  unfold Op at 1.
+  rewrite exec_equiv_bind_bind.
+  rewrite hitrace_incl_opcall.
+  rewrite exec_equiv_bind_bind.
+  rewrite hitrace_incl_opexec.
+  eapply hitrace_incl_bind_a; intros.
+  rewrite hitrace_incl_opret.
+  reflexivity.
 Qed.
